assembler/MemoryAgree.v
@@ -286,42 +286,6 @@ Proof.
 Qed.
 (* end of copy *)
 
-Lemma compare_ints_inject: forall j v1 v2 v1' v2' rs rs' m m',
-    Val.inject j v1 v1' -> Val.inject j v2 v2' ->
-    magree j m m' ->
-    regset_inject j rs rs' -> 
-    regset_inject j (compare_ints v1 v2 rs m) (compare_ints v1' v2' rs' m').
-Proof.
-  intros. unfold compare_ints, Asm.compare_ints.
-  repeat apply regset_inject_expand; auto.
-  - apply cmpu_inject; auto.
-  - apply cmpu_inject; auto.
-  - apply val_negative_inject. apply Val.sub_inject; auto.
-  - apply sub_overflow_inject; auto.
-Qed.
-
-Lemma compare_longs_inject: forall j v1 v2 v1' v2' rs rs' m m',
-    Val.inject j v1 v1' -> Val.inject j v2 v2' ->
-    magree j m m' ->
-    regset_inject j rs rs' -> 
-    regset_inject j (compare_longs v1 v2 rs m) (compare_longs v1' v2' rs' m').
-Proof.
-  intros. unfold compare_longs, Asm.compare_longs.
-  repeat apply regset_inject_expand; auto.
-  - unfold Val.cmplu.
-    exploit (cmplu_bool_lessdef j v1 v2 v1' v2' m m' Ceq); eauto. intros.
-    inversion H3; subst.
-    + simpl. auto. 
-    + simpl. apply Val.vofbool_inject.
-  - unfold Val.cmplu.
-    exploit (cmplu_bool_lessdef j v1 v2 v1' v2' m m' Clt); eauto. intros.
-    inversion H3; subst.
-    + simpl. auto. 
-    + simpl. apply Val.vofbool_inject.
-  - apply val_negativel_inject. apply Val.subl_inject; auto.
-  - apply subl_overflow_inject; auto.
-Qed.
-
 
 (** Preservation of loads *)
 
