assembler/RelocProgGlobalenvs.v
@@ -74,3 +74,5 @@ Definition find_instr (ge: t) (v:val) : option instruction :=
 End GENV.
 
 End Genv.
+
+Coercion Genv.genv_senv: Genv.t >-> Senv.t.
