x86/SymbtablegenproofArchi.v
@@ -57,4 +57,278 @@ Proof.
 Qed.
 
 
+(* set hypothesis *)
+Lemma transf_initial_states : forall rs st1,
+    RealAsm.initial_state prog st1 ->
+    exists st2, initial_state instr_size tprog rs st2 /\ match_states st1 st2.
+Proof.
+  intros rs st1 INIT.
+  generalize TRANSF. intros TRANSF'.
+  unfold match_prog in TRANSF'. unfold transf_program in TRANSF'.
+  destruct (check_wellformedness prog) eqn:WF. 2: congruence. destr_in TRANSF'. 
+  inv INIT.
+  exploit (init_mem_pres_inject m0);eauto.
+  intros (m0' & INITM' & MINJ).
+  (* exploit (Mem.alloc_parallel_inject (Mem.flat_inj (Mem.support m0)) *)
+  (*              m0 m0' 0 (max_stacksize + align (size_chunk Mptr) 8) *)
+  (*              m1 stk 0 (max_stacksize + align (size_chunk Mptr) 8));eauto;try lia. *)
+  exploit (Mem.valid_new_block m0);eauto. unfold Mem.valid_block. intros VALIDSTK.
+  caseEq (Mem.alloc m0' 0 (max_stacksize + align (size_chunk Mptr) 8)).
+  intros m1'  stk'  H0'.
+  exploit (alloc_stack_pres_inject m0 m0');eauto.
+  intros (MINJ1 &  STK &  MATINJ1). subst.  
+  exploit (storev_pres_match_inj Mptr m1 m2);eauto.
+  intros MATINJ2.
+  edestruct storev_pres_inject as (m2' & ST & SMINJ). apply H1. apply MINJ1. econstructor. econstructor.
+  (* stk' is valid *)
+  unfold Mem.flat_inj. destruct (Mem.sup_dec stk' (Mem.support m1)).
+  eauto. congruence.
+  eapply eq_refl. constructor.
+  (* regset *)
+  set (rs0' := rs # PC <- (Genv.symbol_address tge tprog.(prog_main) Ptrofs.zero)
+           # RA <- Vnullptr
+           # RSP <- (Vptr stk' (Ptrofs.sub (Ptrofs.repr (max_stacksize + align (size_chunk Mptr) 8)) (Ptrofs.repr (size_chunk Mptr))))) in *.
+
+  (* instantiate the initial state*)
+  exists (State rs0' m2').
+  split. 
+  (* initial_state *)
+  - econstructor;eauto.
+    econstructor;eauto.
+  - econstructor;eauto.
+    unfold regset_inject. intros.
+    
+    unfold rs0',rs0.
+    apply val_inject_set.
+    apply val_inject_set.
+    apply val_inject_set.
+    auto.
+      (* main function *)
+      destr_in TRANSF'. simpl.
+     exploit (agree_inj_globs (Mem.flat_inj (Mem.support m2)) MATINJ2 ((AST.prog_main prog)) bmain). auto.
+     intros (bmain' & ofs' & MAIN' & MAININJ).
+     (* proof bmain is valid in m2 support *)
+     exploit (Genv.find_symbol_not_fresh). apply H. apply H2. intros VALIDMAIN0.
+     exploit (Mem.valid_block_alloc). apply H0. apply VALIDMAIN0. intros VALIDMAIN1.
+     exploit (Mem.support_store). apply H1. intros SUPEQ.
+     unfold Mem.valid_block in VALIDMAIN1.
+     rewrite <- SUPEQ in VALIDMAIN1. unfold Mem.flat_inj in MAININJ.
+     destruct (Mem.sup_dec bmain (Mem.support m2));try congruence.
+     destr_in MAININJ.
+     unfold Genv.symbol_address.
+     rewrite MAIN'. econstructor.
+     unfold Mem.flat_inj. destruct (Mem.sup_dec bmain' (Mem.support m2));try congruence. eauto.
+     rewrite Ptrofs.add_unsigned. rewrite Ptrofs.add_zero.
+     rewrite <- H6. rewrite Z.add_0_r. rewrite Ptrofs.unsigned_zero. auto.
+     constructor.
+     cbn [Val.offset_ptr].
+     rewrite Ptrofs.sub_add_opp.
+     econstructor.
+     (* prove SSAsm.stkblock = stk' = stk *)
+     exploit (Genv.init_mem_stack). eapply H. intros.
+     exploit (init_mem_stack). eapply INITM'. intros.
+     assert (stk' = SSAsm.stkblock).
+     exploit Mem.alloc_result. eapply H0.
+     unfold Mem.nextblock. unfold Mem.fresh_block. rewrite H3.
+     simpl. intros. rewrite H5. unfold SSAsm.stkblock. auto.
+     (* prove stk' in support m2 *)
+     rewrite <- H5.
+     exploit Mem.support_storev. apply H1. intros.
+     rewrite <- H6. unfold Mem.flat_inj.
+     destruct Mem.sup_dec. eauto.
+     congruence.
+     rewrite Ptrofs.add_zero. auto.
+     (* glob block valid *)
+     
+     unfold glob_block_valid. intros.
+     exploit (Genv.find_def_not_fresh). apply H. apply H3.
+     unfold Mem.valid_block. intros.
+     exploit Mem.support_alloc. apply H0. 
+     exploit Mem.support_storev. apply H1.
+     intros. rewrite <- H5. rewrite H6.
+     exploit Mem.sup_include_incr. apply H4. auto.
+Qed.
+
+
+(* dependent to x86 *)
+Lemma eval_addrmode32_inject: forall j a rs1 rs2,
+    match_inj j ->
+    regset_inject j rs1 rs2 ->
+    Val.inject j (Asm.eval_addrmode32 ge a rs1) (eval_addrmode32 tge a rs2).
+Proof.
+  intros. unfold Asm.eval_addrmode32, eval_addrmode32.
+  destruct a. 
+  destruct base, ofs, const; simpl in *. 
+  - destruct p. repeat apply Val.add_inject; auto.
+    destr_pair_if; auto.
+    apply mul_inject; auto.
+  - destruct p,p0. repeat apply Val.add_inject; auto.
+    destr_pair_if; auto.
+    apply mul_inject; auto.
+    apply inject_symbol_address. auto.
+  - repeat apply Val.add_inject; auto.
+  - destruct p. apply Val.add_inject; auto. 
+    inject_match. apply inject_symbol_address; auto.
+    destruct Archi.ptr64 eqn:PTR.
+    destr_valinj_left H1; inv H1; auto.
+    (* 32bit need the following proof *)
+    destr_valinj_left H1; inv H1; auto.
+    (* destr_pair_if. auto. *)
+    eapply Val.inject_ptr; eauto.
+    repeat unfold Ptrofs.of_int.
+    repeat rewrite Int.unsigned_zero.
+    repeat rewrite Ptrofs.add_zero. auto.
+  - destruct p.
+    inject_match.
+    apply Val.add_inject; auto.
+    destr_pair_if; auto.
+    apply mul_inject; auto.
+    destruct Archi.ptr64 eqn:PTR.
+    destr_valinj_left H1; inv H1; auto.
+
+    destr_valinj_left H1; inv H1; auto.
+    (* destr_pair_if. auto. *)
+    eapply Val.inject_ptr; eauto.
+    repeat unfold Ptrofs.of_int.
+    repeat rewrite Int.unsigned_zero.
+    repeat rewrite Ptrofs.add_zero. auto.
+  - destruct p,p0.
+    inject_match.
+    apply Val.add_inject; auto.
+    destr_pair_if; auto.
+    apply mul_inject; auto.
+    apply inject_symbol_address; auto.
+    destruct Archi.ptr64 eqn:PTR.
+    destr_valinj_left H1; inv H1; auto.
+
+    destr_valinj_left H1; inv H1; auto.
+    destr_pair_if. auto.
+    eapply Val.inject_ptr; eauto.
+    repeat unfold Ptrofs.of_int.
+    repeat rewrite Int.unsigned_zero.
+    repeat rewrite Ptrofs.add_zero. auto.
+  - repeat apply Val.add_inject; auto.
+  - destruct p. 
+    inject_match. inject_match.
+    apply inject_symbol_address; auto.
+    destruct Archi.ptr64 eqn:PTR.    
+    destr_valinj_left H1;inv H1; auto.
+
+    destr_valinj_left H1;inv H1; auto.
+    destr_pair_if. auto.
+    eapply Val.inject_ptr; eauto.
+    repeat unfold Ptrofs.of_int.
+    repeat rewrite Int.unsigned_zero.
+    repeat rewrite Ptrofs.add_zero. auto.
+
+    destruct Archi.ptr64 eqn:PTR.    
+    destr_valinj_left H1; inv H1; auto.
+    destr_valinj_left H1; inv H1; auto.
+    destr_pair_if. auto.
+    eapply Val.inject_ptr; eauto.
+    repeat unfold Ptrofs.of_int.
+    repeat rewrite Int.unsigned_zero.
+    repeat rewrite Ptrofs.add_zero. auto.   
+
+        
+Qed.
+
+    (* destr_pair_if. auto. *)
+    (* eapply Val.inject_ptr; eauto. *)
+    (* repeat unfold Ptrofs.of_int.  *)
+    (* repeat rewrite Int.unsigned_zero.  *)
+    (* repeat rewrite Ptrofs.add_zero. auto. *)
+    (* destr_valinj_left H1; inv H1; auto. *)
+    (* destr_pair_if. auto. *)
+    (* eapply Val.inject_ptr; eauto. *)
+    (* repeat unfold Ptrofs.of_int.  *)
+    (* repeat rewrite Int.unsigned_zero.  *)
+    (* repeat rewrite Ptrofs.add_zero. auto. *)   
+
+Lemma eval_addrmode64_inject: forall j a rs1 rs2,
+    match_inj j ->
+    regset_inject j rs1 rs2 ->
+    Val.inject j (Asm.eval_addrmode64 ge a rs1) (eval_addrmode64 tge a rs2).
+Proof.
+  intros. 
+  destruct a. 
+  destruct base, ofs, const; simpl in *.
+  - destruct p. repeat apply Val.addl_inject; auto.
+    destr_pair_if; auto.
+
+    apply Val.mull_inject; auto.
+  - destruct p,p0. repeat apply Val.addl_inject; auto.
+    destr_pair_if; auto.
+    apply Val.mull_inject; auto.
+    apply inject_symbol_address. auto.
+  - repeat apply Val.addl_inject; auto.
+  - destruct p. apply Val.addl_inject; auto.
+    inject_match.
+    (* dependent in ptr64 !! try to fix it !!!*)
+    apply inject_symbol_address; auto.
+    destruct Archi.ptr64 eqn:PTR.
+    (* 64 *)
+    + destr_valinj_left H1; inv H1;eauto.
+      eapply Val.inject_ptr; eauto.
+      repeat rewrite Ptrofs.add_assoc.
+      rewrite (Ptrofs.add_commut (Ptrofs.repr delta) (Ptrofs.of_int64 Int64.zero)). auto.
+    + destr_valinj_left H1; inv H1;eauto.
+  - destruct p.
+    inject_match.
+    apply Val.addl_inject; auto.
+    destr_pair_if; auto.
+    apply Val.mull_inject; auto.
+    destruct Archi.ptr64 eqn:PTR.
+    (* 64 *)
+    + destr_valinj_left H1; inv H1;eauto.
+      eapply Val.inject_ptr; eauto.
+      repeat rewrite Ptrofs.add_assoc.
+      rewrite (Ptrofs.add_commut (Ptrofs.repr delta) (Ptrofs.of_int64 Int64.zero)). auto.
+    + destr_valinj_left H1; inv H1;eauto.
+  - destruct p,p0.
+    inject_match.
+    apply Val.addl_inject; auto.
+    destr_pair_if; auto.
+    apply Val.mull_inject; auto.
+    apply inject_symbol_address; auto.
+    destruct Archi.ptr64 eqn:PTR.
+    (* 64 *)
+    + destr_valinj_left H1; inv H1;eauto.
+      eapply Val.inject_ptr; eauto.
+      repeat rewrite Ptrofs.add_assoc.
+      rewrite (Ptrofs.add_commut (Ptrofs.repr delta) (Ptrofs.of_int64 Int64.zero)). auto.
+    + destr_valinj_left H1; inv H1;eauto.
+  - repeat apply Val.addl_inject; auto.
+  - destruct p. inject_match. inject_match.
+    apply inject_symbol_address; auto.
+    * destruct Archi.ptr64 eqn:PTR.
+    (* 64 *)
+    + destr_valinj_left H1; inv H1;eauto.
+      eapply Val.inject_ptr; eauto.
+      repeat rewrite Ptrofs.add_assoc.
+      rewrite (Ptrofs.add_commut (Ptrofs.repr delta) (Ptrofs.of_int64 Int64.zero)). auto.
+    + destr_valinj_left H1; inv H1;eauto.
+    *  destruct Archi.ptr64 eqn:PTR.
+    (* 64 *)
+    + destr_valinj_left H1; inv H1;eauto.
+      eapply Val.inject_ptr; eauto.
+      repeat rewrite Ptrofs.add_assoc.
+      rewrite (Ptrofs.add_commut (Ptrofs.repr delta) (Ptrofs.of_int64 Int64.zero)). auto.
+    + destr_valinj_left H1; inv H1;eauto.
+Qed.
+
+Lemma eval_addrmode_inject: forall j a rs1 rs2,
+    match_inj j ->
+    regset_inject j rs1 rs2 ->
+    Val.inject j (Asm.eval_addrmode ge a rs1) (eval_addrmode tge a rs2).
+Proof.
+  intros. unfold Asm.eval_addrmode, eval_addrmode. destruct Archi.ptr64.
+  + eapply eval_addrmode64_inject; eauto.
+  + eapply eval_addrmode32_inject; eauto.
+Qed.
+
+
 End WITH_INSTR_SIZE.
+
+
+
